declutter.

dp/lcs.dfy
@@ -11,17 +11,7 @@ reads a
                     ==> a[i, j] == 0 
 }
 
-function recLCS(a: seq<char>, b: seq<char>): nat
-requires 0 < |a|
-requires 0 < |b|
-decreases a, b
-{
-    if a[|a|-1] == b[|b|-1] && 1 < |a| == |b|
-    then 1 + recLCS(a[..|a|-1], b[..|b|-1])
-    else 0
-}
-
-function recLCS2(a: array2<char>, i: int, j: int): nat
+function recLCS(a: array2<char>, i: int, j: int): nat
 reads a
 decreases i, j
 requires 0 <= i < a.Length0
@@ -30,22 +20,22 @@ requires 0 <= j < a.Length1
     if i == 0 || j == 0
         then 0
     else if a[i, j] != a[i, j]
-        then if recLCS2(a, i-1, j) > recLCS2(a, i, j-1)
-            then recLCS2(a, i-1, j)
-            else recLCS2(a, i, j-1)
+        then if recLCS(a, i-1, j) > recLCS(a, i, j-1)
+            then recLCS(a, i-1, j)
+            else recLCS(a, i, j-1)
         else if a[i, j] == a[i, j]
-            then if recLCS2(a, i-1, j) > recLCS2(a, i, j-1) && recLCS2(a, i-1, j) > 1 + recLCS2(a, i-1, j-1)
-                then recLCS2(a, i-1, j)
-                else if recLCS2(a, i, j-1) > recLCS2(a, i-1, j) && recLCS2(a, i, j-1) > 1 + recLCS2(a, i-1, j-1)
-                    then recLCS2(a, i, j-1)
-                    else 1 + recLCS2(a, i-1, j-1)
+            then if recLCS(a, i-1, j) > recLCS(a, i, j-1) && recLCS(a, i-1, j) > 1 + recLCS(a, i-1, j-1)
+                then recLCS(a, i-1, j)
+                else if recLCS(a, i, j-1) > recLCS(a, i-1, j) && recLCS(a, i, j-1) > 1 + recLCS(a, i-1, j-1)
+                    then recLCS(a, i, j-1)
+                    else 1 + recLCS(a, i-1, j-1)
             else 0
 }
 
 method dpLCS(s: array2<char>, lcsMatrix: array2<nat>) returns (lcsLen: nat)
 requires 0 < lcsMatrix.Length0 && 0 < lcsMatrix.Length1
 requires validMatrix(lcsMatrix)
-ensures s.Length0-1 > 0 && s.Length1-1 > 0 ==> lcsLen == recLCS2(s, s.Length0-1, s.Length1-1)
+ensures s.Length0-1 > 0 && s.Length1-1 > 0 ==> lcsLen == recLCS(s, s.Length0-1, s.Length1-1)
 {
-    assume s.Length0-1 > 0 && s.Length1-1 > 0 ==> lcsLen == recLCS2(s, s.Length0-1, s.Length1-1);
+    assume s.Length0-1 > 0 && s.Length1-1 > 0 ==> lcsLen == recLCS(s, s.Length0-1, s.Length1-1);
 }
